# Problem 11: Gambler’s Ruin

Consider a gambler who at each play of the game has probability $p$ of winning one unit and probability $q = 1-p$ of losing one unit. Assuming that successive plays of the game are independent, what is the probability that, starting with $i$ units, the gambler’s fortune will reach $N$ before reaching $0$?

````{dropdown} Click to show solution

Let $P_i$ be the probability that the gambler, starting with $i$ dollars ($0 < i < N$), reaches $N$ before hitting $0$. We wish to compute $P_i$ under the assumptions that:

- Each play is independent
- The gambler wins 1 unit with probability $p$, and loses 1 unit with probability $q = 1 - p$.

\medskip  
**Step 1: Recurrence relation.**

By conditioning on the outcome of the first game, we obtain:

$$
P_i = pP_{i+1} + qP_{i-1}, \quad \text{for } 1 \le i \le N - 1.
$$

with boundary conditions:

$$
P_0 = 0, \quad P_N = 1.
$$

Rewriting the recurrence:

$$
p(P_{i+1} - P_i) = q(P_i - P_{i-1}) \quad \Longrightarrow \quad P_{i+1} - P_i = r(P_i - P_{i-1}),
$$

where we define \( r := \frac{q}{p} \).

\medskip  
**Step 2: Solve the recurrence.**

This is a linear non-homogeneous recurrence of first differences. Define \( \Delta_i := P_i - P_{i-1} \). Then the recurrence becomes:

$$
\Delta_{i+1} = r \Delta_i.
$$

By induction, it follows that:

$$
\Delta_i = r^{i-1} \Delta_1 = r^{i-1} (P_1 - P_0) = r^{i-1} P_1.
$$

Summing the differences:

$$
P_i = P_0 + \sum_{j=1}^{i} \Delta_j = \sum_{j=1}^{i} r^{j-1} P_1 = P_1 \cdot \sum_{j=0}^{i-1} r^j.
$$

This is a geometric series, so:

$$
P_i = \begin{cases}
    P_1 \cdot \frac{1 - r^i}{1 - r} & \text{if } r \ne 1, \\
    i P_1 & \text{if } r = 1.
\end{cases}
$$

\medskip  
**Step 3: Apply boundary condition \( P_N = 1 \).**

Using the same formula for \( P_N \):

$$
P_N = \begin{cases}
    P_1 \cdot \frac{1 - r^N}{1 - r} = 1 & \text{if } r \ne 1, \\
    N P_1 = 1 & \text{if } r = 1.
\end{cases}
$$

Solving for \( P_1 \), we find:

$$
P_1 = \begin{cases}
    \frac{1 - r}{1 - r^N} & \text{if } r \ne 1, \\
    \frac{1}{N} & \text{if } r = 1.
\end{cases}
$$

Substituting into the expression for \( P_i \), we get the final result:

$$
P_i = \begin{cases}
    \displaystyle\frac{1 - r^i}{1 - r^N} & \text{if } p \ne q, \\
    \displaystyle\frac{i}{N} & \text{if } p = q = \frac{1}{2}, 
\end{cases}
$$

which written in terms of the original variables is 

$$
\boxed{P_i = \begin{cases}
    \displaystyle\frac{1 - (q/p)^i}{1 - (q/p)^N} & \text{if } p \ne q, \\
    \displaystyle\frac{i}{N} & \text{if } p = q = \frac{1}{2}.
\end{cases}}
$$

````
