# Problem 17: Streak Freak

Let $(X_t)_{t \ge 1}$ be a sequence of independent Bernoulli random variables, where $\mathbb{P}(X_t = 1) = p$ and $\mathbb{P}(X_t = 0) = 1 - p$, for a fixed $p \in (0,1)$. Define $T_k$ to be the first time $t$ such that the sequence $(X_{t-k+1}, X_{t-k+2}, \ldots, X_t)$ consists of $k$ consecutive successes (i.e., $X_{t-k+1} = X_{t-k+2} = \cdots = X_t = 1$). Compute the expected value $\mathbb{E}[T_k]$.

````{dropdown} Click to show solution

Let $E_i$ denote the expected number of experiments (or moves) to first get $i$ consecutive successes. To obtain $i$ successes we first need to have $(i-1)$ consecutive successes and then consider the next experiment. If the experiment is a success (with probability $p$), we have achieved $i$ consecutive successes and the cost is $1$ (the experiment itself). If it is a failure (with probability $1-p$), the run is broken and we must start all over, costing an additional $E_i$ moves. This leads to the recurrence:

$$
E_i = E_{i-1} + p \cdot 1 + (1-p) \cdot E_i.
$$

Rearranging:

$$
E_i - (1-p)E_i = E_{i-1} + p,
$$

or equivalently:

$$
p\,E_i = E_{i-1} + p.
$$

Dividing both sides by $p$:

$$
E_i = \frac{1}{p} + \frac{1}{p}E_{i-1}.
$$

With the base case $E_0 = 0$ (since zero successes in a row require no moves), we can solve this recurrence by iteration. For instance:

$$
\begin{aligned}
E_1 &= \frac{1}{p} + \frac{1}{p}E_0 = \frac{1}{p},\\
E_2 &= \frac{1}{p} + \frac{1}{p}E_1 = \frac{1}{p} + \frac{1}{p^2},\\
E_3 &= \frac{1}{p} + \frac{1}{p}E_2 = \frac{1}{p} + \frac{1}{p^2} + \frac{1}{p^3},\\
&\;\vdots\\
E_k &= \frac{1}{p} + \frac{1}{p^2} + \cdots + \frac{1}{p^k}.
\end{aligned}
$$

Thus, the expected number of moves required to obtain $k$ consecutive successes is:

$$
\boxed{
E_k = \frac{1}{p} + \frac{1}{p^2} + \cdots + \frac{1}{p^k} = \frac{1 - p^k}{p^k(1 - p)}.
}
$$

````
