# Problem 4: Hat Party

Suppose $n$ men at a party throw their hats in the center of the room. Each man then randomly selects a hat. Let $p_n$ be the probability that none of the $n$ men selects his own hat. What is $\lim\limits_{n\to \infty}p_n$?

````{dropdown} Click to show solution

Consider $n$ men labeled $1,2,\dots,n$ and hats labeled identically. Each man randomly chooses a hat from the center. We want the probability $p_n$ that no man selects his own hat.

---

### Step 1: Formalizing the Problem

This is equivalent to counting permutations. Define the set of all permutations of $\{1,\dots,n\}$ as $\mathbb{S}_n$, with $|\mathbb{S}_n| = n!$. Define the events:

$$
E_i = \{\text{the $i$-th person selects his own hat}\}, \quad 1 \leq i \leq n.
$$

Then the event whose probability we wish to compute is:

$$
\bigcap_{i=1}^{n}\overline{E_i}.
$$

Using complementary probability:

$$
p_n = \Pr\left(\bigcap_{i=1}^{n}\overline{E_i}\right) = 1 - \Pr\left(\bigcup_{i=1}^{n} E_i\right).
$$

---

### Step 2: Inclusion–Exclusion Principle

Using the Inclusion–Exclusion Principle:

$$
\Pr\left(\bigcup_{i=1}^{n}E_i\right) = \sum_{1\leq i\leq n}\Pr(E_i) - \sum_{1\leq i<j\leq n}\Pr(E_i\cap E_j) + \cdots + (-1)^{k+1} \sum_{1\leq i_1<\dots<i_k\leq n}\Pr(E_{i_1}\cap\dots\cap E_{i_k}) + \cdots + (-1)^{n+1}\Pr(E_1 \cap \dots E_n)
$$

---

### Step 3: Computing the Probabilities of Intersections

Each permutation is equally likely, so each has probability $1/n!$.

- For a single $i$:

  $$
  \Pr(E_i) = \frac{(n-1)!}{n!} = \frac{1}{n}.
  $$

- For distinct $i,j$:

  $$
  \Pr(E_i \cap E_j) = \frac{(n-2)!}{n!} = \frac{1}{n(n-1)}.
  $$

- More generally, for $k$ distinct indices:

  $$
  \Pr(E_{i_1}\cap\dots\cap E_{i_k}) = \frac{(n-k)!}{n!}.
  $$

There are $\binom{n}{k}$ such index sets, so:

$$
\sum_{1 \leq i_1 < \dots < i_k \leq n} \Pr(E_{i_1} \cap \dots \cap E_{i_k}) = \binom{n}{k} \cdot \frac{(n-k)!}{n!}.
$$

Thus:

$$
\Pr\left(\bigcup_{i=1}^{n} E_i \right) = \sum_{k=1}^n (-1)^{k+1} \binom{n}{k} \cdot \frac{(n-k)!}{n!}.
$$

---

### Step 4: Simplifying the Expression

Note:

$$
\binom{n}{k} \cdot \frac{(n-k)!}{n!} = \frac{n!}{k!(n-k)!} \cdot \frac{(n-k)!}{n!} = \frac{1}{k!}.
$$

Therefore:

$$
\Pr\left(\bigcup_{i=1}^{n} E_i \right) = \sum_{k=1}^n (-1)^{k+1} \cdot \frac{1}{k!},
$$

and hence:

$$
p_n = 1 - \sum_{k=1}^n (-1)^{k+1} \cdot \frac{1}{k!} = \frac{1}{2!} - \frac{1}{3!} + \frac{1}{4!} - \cdots + (-1)^n \cdot \frac{1}{n!}.
$$

---

### Step 5: Taking the Limit

We now compute:

$$
\lim_{n \to \infty} p_n = \lim_{n \to \infty} \left( \frac{1}{2!} - \frac{1}{3!} + \frac{1}{4!} - \cdots + (-1)^n \cdot \frac{1}{n!} \right).
$$

Recall the Taylor series for $e^{-1}$:

$$
e^{-1} = 1 - \frac{1}{1!} + \frac{1}{2!} - \frac{1}{3!} + \cdots
$$

So:

$$
\frac{1}{2!} - \frac{1}{3!} + \cdots = e^{-1} - 1 + \frac{1}{1!} = e^{-1}.
$$

Hence:

$$
\lim_{n \to \infty} p_n = \boxed{e^{-1}}.
$$

````
