# Problem 3: Stairway to Random

Let $n$ be a positive integer.  Set $a_{n, 0}=1$. For $k\geq 0$, choose an integer $m_{n, k}$ uniformly at random from the set $\{1, . . . , n\}$, and let

$$
a_{n, k+1} = \begin{cases}
    a_{n, k}+1 & \text{if }m_{n, k} > a_{n, k}\\
    a_{n, k} & \text{if }m_{n, k} = a_{n, k}\\
    a_{n, k}-1 & \text{if }m_{n, k} < a_{n, k}.
\end{cases}
$$

Let $E(n)$ be the expected value of $a_{n, n}$. Determine the value of $\lim_{n\to \infty} E(n)/n$

````{dropdown} Click to show solution

Fix $n$ first. For $k \geq 0$, define $E_k = \mathbb{E}[a_{n,k}], \text{with the initial condition } a_{n,0}=1.$ We start by conditioning on the random variable $a_{n,k}$ to find a recurrence relation for $E_k$. Using the given recurrence definition of $a_{n,k}$ and the distribution of $m_{n,k}$, we have

$$
\mathbb{E}[a_{n,k+1}\mid a_{n,k}] 
= \frac{n - a_{n,k}}{n}(a_{n,k} + 1) + \frac{1}{n}a_{n,k} + \frac{a_{n,k} - 1}{n}(a_{n,k}-1).
$$

Expanding and simplifying the right-hand side algebraically gives:

$$
\begin{aligned}
\mathbb{E}[a_{n,k+1}\mid a_{n,k}]
&= \frac{(n - a_{n,k})(a_{n,k}+1) + a_{n,k} + (a_{n,k}-1)^2}{n} \\[5pt]
&= \frac{(n a_{n,k}+ n - a_{n,k}^2 - a_{n,k}) + a_{n,k} + (a_{n,k}^2 - 2a_{n,k}+1)}{n} \\[5pt]
&= \frac{n a_{n,k}+ n - a_{n,k}^2 - a_{n,k} + a_{n,k} + a_{n,k}^2 - 2a_{n,k}+1}{n} \\[5pt]
&= \frac{n a_{n,k}+ n - 2 a_{n,k}+1}{n} \\[5pt]
&= \left(1-\frac{2}{n}\right)a_{n,k}+1+\frac{1}{n}.
\end{aligned}
$$

Now, recall the law of total expectation, which states for random variables $X$ and $Y$: $\mathbb{E}[X] = \mathbb{E}[\mathbb{E}[X\mid Y]].$ Applying this law, we find a recurrence relation for the sequence $E_k$:

$$
\begin{aligned}
E_{k+1} 
&= \mathbb{E}[a_{n,k+1}] \\[5pt]
&= \mathbb{E}[\mathbb{E}[a_{n,k+1}\mid a_{n,k}]] \\[5pt]
&= \mathbb{E}\left[ \left(1-\frac{2}{n}\right)a_{n,k}+1+\frac{1}{n} \right] \\[5pt]
&= \left(1-\frac{2}{n}\right)\mathbb{E}[a_{n,k}] + 1+\frac{1}{n} \\[5pt]
&= \left(1-\frac{2}{n}\right)E_k + 1+\frac{1}{n}.
\end{aligned}
$$

This linear recurrence relation, together with the initial condition $E_0 = a_{n,0} = 1$, is given explicitly as:

$$
E_{k+1} = \left(1-\frac{2}{n}\right)E_k + 1+\frac{1}{n}, \quad E_0 = 1.
$$

**Solving the recurrence:**

This is a non-homogeneous linear recurrence relation. To solve it, we use standard methods from linear recurrence theory.

**Step 1 (Solve the homogeneous recurrence):**  
Consider the associated homogeneous recurrence:

$$
E_{k+1}^{(h)} = \left(1-\frac{2}{n}\right)E_k^{(h)}.
$$

Its general solution is straightforward:

$$
E_k^{(h)} = C\left(1-\frac{2}{n}\right)^k
$$

for some constant $C$ determined later.

**Step 2 (Find a particular solution):**  
Because the non-homogeneous term is constant ($1+\frac{1}{n}$), we try a constant particular solution $E_k^{(p)} = A$. Substitute this into the recurrence:

$$
A = \left(1-\frac{2}{n}\right)A + 1+\frac{1}{n}.
$$

Solve for $A$:

$$
A - \left(1-\frac{2}{n}\right)A = 1+\frac{1}{n} \quad\Rightarrow\quad A\left(\frac{2}{n}\right)=1+\frac{1}{n}.
$$

Thus:

$$
A = \frac{1+\frac{1}{n}}{\frac{2}{n}} = \frac{n+1}{2}.
$$

Thus a particular solution is:

$$
E_k^{(p)} = \frac{n+1}{2}.
$$

**Step 3 (General solution):**  
The full general solution to our recurrence is thus:

$$
E_k = E_k^{(h)} + E_k^{(p)} = C\left(1-\frac{2}{n}\right)^k + \frac{n+1}{2}.
$$

**Step 4 (Apply initial conditions):**  
Use $E_0=1$ to determine the constant $C$:

$$
E_0 = C\left(1-\frac{2}{n}\right)^0 + \frac{n+1}{2} = C + \frac{n+1}{2}=1.
$$

Solve for $C$:

$$
C = 1 - \frac{n+1}{2} = \frac{1-n}{2}.
$$

Thus, the explicit solution for the recurrence is:

$$
E_k = \frac{1-n}{2}\left(1-\frac{2}{n}\right)^k + \frac{n+1}{2}.
$$

**Evaluate at $k=n$:**  
Substituting $k=n$, we get the explicit form for $E(n) = E_n$:

$$
E(n)=E_n=\frac{1-n}{2}\left(\frac{n-2}{n}\right)^n + \frac{n+1}{2}.
$$

**Compute the limit as $n\to\infty$:**  
We finally compute:

$$
\begin{aligned}
\lim_{n\to\infty}\frac{E(n)}{n}
&=\lim_{n\to\infty}\frac{1}{n}\left[\frac{1-n}{2}\left(1-\frac{2}{n}\right)^n+\frac{n+1}{2}\right] \\[5pt]
&=\frac{1}{2}\lim_{n\to\infty}\left[\frac{1-n}{n}\left(1-\frac{2}{n}\right)^n+1+\frac{1}{n}\right] \\[5pt]
&=\frac{1}{2}\left[(-1)\cdot e^{-2}+1\right], \quad\text{(since $\lim_{n\to\infty}(1-2/n)^n=e^{-2}$)} \\[5pt]
&=\frac{1-e^{-2}}{2}.
\end{aligned}
$$

Thus, the final answer is:

$$
\boxed{\frac{1-e^{-2}}{2}}.
$$

````
