# Problem 16: Coin Toss Monotony

$n$ players, $P_1, ..., P_n$ are rolling a coin until they get head. Let $X_1, X_2, ..., X_n$ be the number of throws they need respectively. What is $\Pr[X_1\leq X_2 \leq \dots \leq X_n]$?  

*Hint: Do it for $n=1,2,3$, and try to see a pattern.*

````{dropdown} Click to show solution

Let $X_1, X_2, \dots, X_n$ be independent and identically distributed geometric random variables with parameter $p = \frac{1}{2}$, i.e.,  

$$
\mathbb{P}(X_i = k) = \left( \frac{1}{2} \right)^k, \quad k = 1, 2, 3, \dots
$$

We claim that:  

$$
\boxed{
\mathbb{P}(X_1 \le X_2 \le \dots \le X_n) = \left( \frac{1}{2} \right)^n \prod_{k=1}^n \frac{1}{1 - 2^{-k}}
}
$$

---

**Base Case: $n = 1$**

$$
\mathbb{P}(X_1 \le X_1) = 1
$$  

$$
\left( \frac{1}{2} \right)^1 \cdot \frac{1}{1 - 2^{-1}} = \frac{1}{2} \cdot \frac{1}{1 - \frac{1}{2}} = \frac{1}{2} \cdot 2 = 1
$$  

The base case holds.

---

**Inductive Step**

Assume the formula holds for $n$. That is,  

$$
\mathbb{P}(X_1 \le X_2 \le \dots \le X_n) = \left( \frac{1}{2} \right)^n \prod_{k=1}^n \frac{1}{1 - 2^{-k}}
$$

We will prove it holds for $n+1$.

---

**Condition on $X_1 = k$**

$$
\mathbb{P}(X_1 \le X_2 \le \dots \le X_{n+1}) = \sum_{k=1}^\infty \mathbb{P}(X_1 = k) \cdot \mathbb{P}(X_2 \ge k, \dots, X_{n+1} \ge k \text{ and sorted} \mid X_1 = k)
$$

By independence and memorylessness, after conditioning on $X_1 = k$, define:  

$$
Y_i = X_i - k \mid X_i \ge k \sim \text{Geom}(1/2)
$$

Then:  

$$
\mathbb{P}(X_2 \ge k, \dots, X_{n+1} \ge k \text{ and sorted}) = \left(\prod_{2 \leq i \leq n+1} \mathbb{P}(X_i \ge k)\right) \cdot \mathbb{P}(Y_2 \le \dots \le Y_{n+1})
$$  

$$
= \frac{1}{2^{(k-1)n}} \cdot \mathbb{P}(Y_2 \le \dots \le Y_{n+1})
$$

Thus:  

$$
\mathbb{P}(X_1 \le \dots \le X_{n+1}) = \sum_{k=1}^\infty \left( \frac{1}{2} \right)^{k + (k-1)n} \cdot \mathbb{P}(Y_2 \le \dots \le Y_{n+1})
$$

But  

$$
\mathbb{P}(Y_2 \le \dots \le Y_{n+1}) = \left( \frac{1}{2} \right)^n \prod_{k=1}^n \frac{1}{1 - 2^{-k}}
$$

Therefore:  

$$
\mathbb{P}(X_1 \le \dots \le X_{n+1}) = \sum_{k=1}^\infty \left( \frac{1}{2} \right)^{k + (k-1)n} \cdot \left( \frac{1}{2} \right)^n \prod_{r=1}^n \frac{1}{1 - 2^{-r}}
$$  

$$
= \left( \frac{1}{2} \right)^n \prod_{r=1}^n \frac{1}{1 - 2^{-r}} \cdot \sum_{k=1}^\infty \left( \frac{1}{2^{n+1}} \right)^k \cdot \left( \frac{1}{2^{-n}} \right)
$$  

$$
= \left( \frac{1}{2} \right)^n \prod_{r=1}^n \frac{1}{1 - 2^{-r}} \cdot \frac{2^n}{2^{n+1} - 1}
$$  

$$
= \left( \frac{1}{2} \right)^{n+1} \prod_{k=1}^{n+1} \frac{1}{1 - 2^{-k}}
$$

Hence, by induction, the formula holds for all $n \ge 1$.

````
